scm:SeshatChoices 
	a owl:Ontology;
	rdfs:comment "Properties that can only take a specific set of values are enumerated types and defined here for Seshat"@en ;
	rdfs:label "Seshat Enumerated Types"@en.
	
scm:Confidence
	a owl:Class ;
	rdfs:comment "Tags that can be added to values to indicate confidence in the value of some piece data"@en ;
	rdfs:label "Confidence Tags"@en ;
	rdfs:subClassOf tcs:Enumerated ;
	owl:oneOf (
		scm:inferred
		scm:disputed
   		scm:dubious
		scm:uncertain
	) .

scm:EpistemicState
  rdfs:label "Epistemic State"@en ;
  rdfs:comment "The existence of a feature in the historical record"@en ;
  a owl:Class ;
  rdfs:subClassOf tcs:Enumerated ;
  owl:oneOf (
   scm:unknown
   scm:absent
   scm:present
 ) .

scm:EpistemicFrequency
  rdfs:label "Epistemic Frequency"@en ;
  rdfs:comment "The frequency of a feature in the historical record"@en ;
  a owl:Class ;
  rdfs:subClassOf tcs:Enumerated ;
  owl:oneOf (
   scm:unknown_epistemic_frequency
   scm:never
   scm:rare
   scm:frequent
 ) .

scm:DegreeOfCentralization
  rdfs:label "Degree of Centralization"@en ;
  rdfs:comment "An indication of how centralized a political authority was"@en ;
  a owl:Class ;
  rdfs:subClassOf tcs:Enumerated ;
  owl:oneOf (
   scm:quasipolity
   scm:nominal
   scm:loose
   scm:confederated_state
   scm:unitary_state
   scm:unknown_centralization
   scm:no_centralization
 ) .

scm:Change
  rdfs:label "Size of Change"@en ;
  rdfs:comment "How much change has taken place"@en ;
  a owl:Class ;
  rdfs:subClassOf tcs:Enumerated ;
  owl:oneOf (
   scm:unknown_change
   scm:big_decrease
   scm:small_decrease
   scm:stable
   scm:small_increase
   scm:big_increase
 ) .

 scm:ComplexityChange
  rdfs:label "Change in complexity"@en ;
  rdfs:comment "How much change has taken place in complexity"@en ;
  a owl:Class ;
  rdfs:subClassOf tcs:Enumerated ;
  owl:oneOf (
   scm:unknown_complexity_change
   scm:organization_collapses
   scm:complexity_decreases
   scm:stable_complexity
   scm:complexity_increases
   scm:big_complexity_increase
 ) .

scm:SupraPolityRelations
  rdfs:label "Supra-Polity Relations"@en ;
  rdfs:comment "The relationship between a polity and its paramount power "@en ;
  a owl:Class ;
  rdfs:subClassOf tcs:Enumerated ;
  owl:oneOf (
   scm:alliance
   scm:nominal_allegiance
   scm:personal_union
   scm:vassalage
   scm:no_supra_polity_relations
   scm:unknown_supra_polity_relations
 ) .

scm:PoliticalEvolution
  rdfs:label "Political Evolution"@en ;
  rdfs:comment "The ways in which a political authority can evolve into another one"@en ;
  a owl:Class ;
  rdfs:subClassOf tcs:Enumerated ;
  owl:oneOf (
   scm:continuity
   scm:assimilation
   scm:elite_migration
   scm:population_migration
   scm:unknown_evolution
 ) .

scm:IncomeSource
  a owl:Class ;
  rdfs:label "Source of Income"@en ;
  rdfs:comment "A source of income"@en ;
  a owl:Class ;
  rdfs:subClassOf tcs:Enumerated ;
  owl:oneOf (
   scm:state_salary
   scm:governed_population
   scm:land
   scm:no_income
   scm:unknown_income
 ) .

scm:Frequency
	rdfs:label "Frequency"@en ;
	rdfs:comment "The genrational frequencies of events"@en ;
	a owl:Class ;
	rdfs:subClassOf tcs:Enumerated ;
	owl:oneOf (
	scm:daily
	scm:weekly
	scm:monthly
	scm:seasonally
	scm:yearly
	scm:once_per_generation
	scm:once_in_a_lifetime
	scm:unknown_frequency
) .

scm:AuthorityEmphasis
	rdfs:label "Authority Emphasis"@en ;
	rdfs:comment "Group Authority Emphasis - from leader to collective"@en ;
	a owl:Class ;
	rdfs:subClassOf tcs:Enumerated ;
	owl:oneOf (
		scm:egalitarian
		scm:group_solidarity
		scm:group_priority
		scm:leader_priority
		scm:leader_emphasis
		scm:unknown_emphasis
	) .

scm:AuthoritySharing
	rdfs:label "Authority Sharing"@en ;
	rdfs:comment "The sharing of authority"@en ;
	a owl:Class ;
	rdfs:subClassOf tcs:Enumerated ;
	owl:oneOf (
		scm:egalitarian_sharing
		scm:extensive_sharing
		scm:cadre_sharing
		scm:rare_sharing
		scm:exclusive_sharing
		scm:unknown_sharing
	) .

scm:ExternalContact
	rdfs:label "External Contact"@en ;
	rdfs:comment "Particiption in external contacts"@en ;
	a owl:Class ;
	rdfs:subClassOf tcs:Enumerated ;
	owl:oneOf (
		scm:egalitarian_contact
		scm:few_contacts
		scm:nonexclusive_leader_participation
		scm:nonexclusive_leader_control
		scm:exclusive_leader_control
		scm:unknown_contact
	) .

scm:LeaderDifferentiation
	rdfs:label "Leader Differentiation"@en ;
	rdfs:comment "Differentiation among leaders and followers."@en ;
	a owl:Class ;
	rdfs:subClassOf tcs:Enumerated ;
	owl:oneOf (
		scm:egalitarian_differentiation
		scm:no_differentiation
		scm:small_privileges
		scm:extensive_privileges
		scm:exclusive_privileges
		scm:unknown_differentiation
	) .

scm:LeaderIdentification
	rdfs:label "Leader Indentification"@en ;
	rdfs:comment "Mechanisms by which a leader is identified"@en ;
	a owl:Class ;
	rdfs:subClassOf tcs:Enumerated ;
	owl:oneOf (
		scm:no_leader
		scm:egalitarian_leadership
		scm:leader_treatment
		scm:leader_symbols
		scm:leader_cult
		scm:unknown_identification
	) .

scm:Standardization
  rdfs:label "Standardization"@en ;
  rdfs:comment "The standard nature of a feature"@en ;
  a owl:Class ;
  rdfs:subClassOf tcs:Enumerated ;
  owl:oneOf (
	scm:unknown_standardization
	scm:no_standardization
	scm:unstandardized
	scm:moderately_unstandardized
	scm:moderately_standardized
	scm:standardized
 ) .

scm:daily
	rdfs:label "Daily"@en ;
	rdfs:comment "Occuring every day (or most days)"@en ;
	a scm:Frequency .

scm:weekly
	rdfs:label "Weekly"@en ;
	rdfs:comment "Occurring once per week (or similar frequency)"@en ;
	a scm:Frequency .

scm:monthly
	rdfs:label "Monthly"@en ;
	rdfs:comment "Occurring once per month (or similar frequency)"@en ;
	a scm:Frequency .

scm:seasonally
	rdfs:label "Seasonally"@en ;
	rdfs:comment "Occurring 4 times per year (or similar frequency)"@en 
	a tcs:Frequency.

scm:yearly
	rdfs:label "Yearly"@en ;
	rdfs:comment "Occurring once a year (or similar frequency)"@en ;
	a scm:Frequency .

scm:once_per_generation
	rdfs:label "Once per generation"@en ;
	rdfs:comment "Occurring once a generation (20 years or similar frequency)"@en ;
	a scm:Frequency .

scm:once_in_a_lifetime
	rdfs:label "Once in a lifetime"@en ;
	rdfs:comment "Occurring once in an individual's lifetime"@en ;
	a scm:Frequency .

scm:egalitarian
	rdfs:label "Egalitarian"@en ;
	rdfs:comment "Egalitarian / no formal leaders"@en ;
	a scm:AuthorityEmphasis.

scm:group_solidarity
	rdfs:label "Group Solidarity"@en ;
	rdfs:comment "emphasis placed on group solidarity and group survival "@en ;
	a scm:AuthorityEmphasis .

scm:group_priority
	rdfs:label "Group Priority"@en ;
	rdfs:comment "emphasis shared between group and leader, with greatest importance given to group survival"@en ;
	a scm:AuthorityEmphasis .

scm:leader_priority
	rdfs:label "Leader Priority"@en ;
	rdfs:comment "emphasis shared between group and leader, with greatest importance given to leader survival "@en ;
	a scm:AuthorityEmphasis .

scm:leader_emphasis
	rdfs:label "Leader Emphasis"@en ;
	rdfs:comment "emphasis placed on leaders as the embodiment of the group"@en ;
	a scm:AuthorityEmphasis .

scm:extensive_sharing
	rdfs:label "Extensive Sharing"@en ;
	rdfs:comment "leaders share power extensively with others "@en ;
	a scm:AuthoritySharing .

scm:cadre_sharing
	rdfs:label "Cadre Sharing"@en ;
	rdfs:comment "leaders share power with a large cadre of other leaders"@en ;
	a scm:AuthoritySharing .

scm:rare_sharing
	rdfs:label "Rare Sharing"@en ;
	rdfs:comment "leaders share power with a few other leaders "@en ;
	a scm:AuthoritySharing .

scm:exclusive_sharing
	rdfs:label "Exclusive Sharing"@en ;
	rdfs:comment "leaders exercise exclusive power"@en ;
	a scm:AuthoritySharing .

scm:few_contacts
	rdfs:label "Few contacts"@en ;
	rdfs:comment "few or unimportant"@en ;
	a scm:ExternalContact .

scm:nonexclusive_leader_participation
	rdfs:label "Non-exclusive Participation"@en ;
	rdfs:comment "external contacts are part of leaders' authority, but not exclusive"@en ;
	a scm:ExternalContact .

scm:nonexclusive_leader_control
	rdfs:label "Non-exclusive Control"@en ;
	rdfs:comment "external contacts are key to leaders' authority, but not exclusive"@en ;
	a scm:ExternalContact .

scm:exclusive_leader_control
	rdfs:label "Exclusive Control"@en ;
	rdfs:comment "external contacts are exclusively controlled by leaders"@en ;
	a scm:ExternalContact .


scm:no_differentiation
	rdfs:label "No Differentiation"@en ;
	rdfs:comment "No Differentiation"@en ;
	a scm:LeaderDifferentiation .

scm:small_privileges
	rdfs:label "Some Privileges"@en ;
	rdfs:comment "leaders have some privileges and/or access to resources others do not"@en ;
	a scm:LeaderDifferentiation .

scm:extensive_privileges
	rdfs:label "Extensive Privileges"@en ;
	rdfs:comment "leaders have extensive privileges and access to resources others do not, including special housing and sumptuary goods"@en ;
	a scm:LeaderDifferentiation .

scm:exclusive_privileges
	rdfs:label "Exclusive Privileges"@en ;
	rdfs:comment "lleaders have exclusive privileges and exclusive access to special housing, resources, and sumptuary goods"@en ;
	a scm:LeaderDifferentiation .

scm:no_standardization
	rdfs:label "None"@en ;
	rdfs:comment "No standardization exists"@en ;
	a scm:Standardization .

scm:leader_treatment
	rdfs:label "Identified by treatment"@en ;
	rdfs:comment "leaders are identified by treatment or appearance"@en ;
	a scm:LeaderIdentification .

scm:leader_symbols
	rdfs:label "Identified by symbols"@en ;
	rdfs:comment "leaders are identified by recognized symbols of power or special behaviors"@en ;
	a scm:LeaderIdentification .

scm:leader_cult
	rdfs:label "cult of leadership"@en ;
	rdfs:comment "individual aggrandizement and/or cult of leaders"@en ;
	a scm:LeaderIdentification .

scm:absent
    a scm:EpistemicState;
    rdfs:comment "The feature was absent in this historical context"@en ;
    rdfs:label "Absent"@en .

scm:active
	a scm:GodType ;
	rdfs:comment "Present and active in human affairs but not supportive of human morality"@en ;
	rdfs:label "Active"@en .

scm:alliance
	a scm:SupraPolityRelations ;
	rdfs:comment "belongs to a long-term military-political alliance of independent polities ('long-term' refers to more or less permanent relationship between polities extending over multiple years"@en ;
	rdfs:label "Alliance"@en .

scm:assimilation
	a scm:PoliticalEvolution ;
	rdfs:comment "Assimilation by another political authority in the absence of substantial population replacement"@en ;
	rdfs:label "Cultural Assimilation"@en .

scm:big_complexity_increase
	a scm:ComplexityChange ;
	rdfs:comment "Radical increase in the size and/or organizational complexity"@en ;
	rdfs:label "Radical Increase"@en .

scm:big_decrease
	a scm:Change ;
	rdfs:comment "Dramatic Decrease"@en ;
	rdfs:label "Dramatic Decrease"@en .

scm:big_increase
	a scm:Change ;
	rdfs:comment "Dramatic Increase"@en ;
	rdfs:label "Dramatic Increase"@en .

scm:complexity_decreases
	a scm:ComplexityChange ;
	rdfs:comment " Size and/or organizational complexity decreases."@en ;
	rdfs:label "Decreased Complexity"@en .

scm:complexity_increases
	a scm:ComplexityChange ;
	rdfs:comment "Size and/or organizational complexity increases."@en ;
	rdfs:label "Increased Complexity"@en .

scm:confederated_state
	a scm:DegreeOfCentralization ;
	rdfs:comment "regions enjoy a large degree of autonomy in internal (regional) government. In particular, the regional governors are either hereditary rulers, or are elected by regional elites or by the population of the region; and regional governments can levy and dispose of regional taxes. Use this category for the more centralized "@en ;
	rdfs:label "Confederated State"@en .

scm:continuity
	a scm:PoliticalEvolution ;
	rdfs:comment "Gradual change without any discontinuity"@en ;
	rdfs:label "Continuity"@en .

scm:elite_migration
	a scm:PoliticalEvolution ;
	rdfs:comment "The preceding elites were replaced by new elites coming from elsewhere"@en ;
	rdfs:label "Elite Migration"@en .

scm:frequent
	a scm:EpistemicFrequency ;
	rdfs:comment "The feature was frequent in the historical context"@en ;
	rdfs:label "Frequent"@en .

scm:governed_population
	a scm:IncomeSource ;
	rdfs:comment "means that the official directly collects tribute from the population (for example, the 'kormlenie' system in Medieval Russia)."@en ;
	rdfs:label "Governed Population"@en .

scm:inactive
	a scm:GodType ;
	rdfs:comment "Present but not active in human affairs"@en ;
	rdfs:label "Inactive"@en .

scm:land
	a scm:IncomeSource ;
	rdfs:comment "Living off land supplied by the state."@en ;
	rdfs:label "Land"@en .

scm:loose
	a scm:DegreeOfCentralization ;
	rdfs:comment "the central government exercises a certain degree of control, especially over military matters and international relations. Otherwise the regional rulers are left alone (example: European "@en ;
	rdfs:label "Loose"@en .

scm:moderately_standardized
	a scm:Standardization ;
	rdfs:comment "Moderately standardized (more standard than not)"@en;
	rdfs:label "Moderately Standardized"@en .

scm:moderately_unstandardized
	a scm:Standardization ;
	rdfs:comment "Moderately Unstandardized (more unstandard than not)"@en;
	rdfs:label "Moderately Unstandardized"@en .

scm:moralizing
	a scm:GodType ;
	rdfs:comment "Present, active, and specifically supportive of human morality"@en ;
	rdfs:label "Moralizing"@en .

scm:no_centralization
	a scm:DegreeOfCentralization ;
	rdfs:comment "There is no centralised system"@en ;
	rdfs:label "None"@en .

scm:no_income
	a scm:IncomeSource ;
	rdfs:comment "The state officials are not compensated (example: in the Republican and Principate Rome the magistrates were wealthy individuals who served without salary, motivated by prestige and social or career advancement)"@en ;
	rdfs:label "None"@en .

scm:no_supra_polity_relations
	a scm:SupraPolityRelations ;
	rdfs:comment "No relations with any supracultural entity"@en ;
	rdfs:label "None"@en .

scm:nominal
	a scm:DegreeOfCentralization ;
	rdfs:comment "regional rulers pay only nominal allegiance to the overall ruler and maintain independence on all important aspects of governing, including taxation and warfare. (example: Japan during the Sengoku period)"@en ;
	rdfs:label "Nominal "@en .

scm:nominal_allegiance
	a scm:SupraPolityRelations ;
	rdfs:comment "ay only nominal allegiance to the overall ruler and maintain independence on all important aspects of governing, including taxation and warfare."@en ;
	rdfs:label "Nominal Allegiance"@en .

scm:organization_collapses
	a scm:ComplexityChange ;
	rdfs:comment "Organization collapses."@en ;
	rdfs:label "Collapse"@en .

scm:personal_union
	a scm:SupraPolityRelations ;
	rdfs:comment "the focal polity is united with another, or others, as a result of a dynastic marriage"@en ;
	rdfs:label "Personal Union"@en .

scm:population_migration
	a scm:PoliticalEvolution ;
	rdfs:comment "Evidence for substantial population replacement"@en ;
	rdfs:label "Population Migration"@en .

scm:present
	a scm:EpistemicState ;
	rdfs:comment "The feature was present in this historical context"@en ;
	rdfs:label "Present"@en .

scm:quasipolity
	a scm:DegreeOfCentralization ;
	rdfs:comment "Use if the NGA is inhabited by many politically independent groups"@en ;
	rdfs:label "Quasi-polity"@en .

scm:rare
	a scm:EpistemicFrequency ;
	rdfs:comment "The feature was rare in the historical context"@en ;
	rdfs:label "Rare"@en .

scm:small_decrease
	a scm:Change ;
	rdfs:comment "Minor Decrease"@en ;
	rdfs:label "Minor Decrease"@en .

scm:small_increase
	a scm:Change ;
	rdfs:comment "Minor Increase"@en ;
	rdfs:label "Minor Increase"@en .

scm:stable
	a scm:Change ;
	rdfs:comment "Stable - no change"@en ;
	rdfs:label "Stable"@en .

scm:stable_complexity
	a scm:ComplexityChange ;
	rdfs:comment " Size and/or organizational complexity remains stable."@en ;
	rdfs:label "Stable"@en .

scm:standardized
	a scm:Standardization ;
	rdfs:comment "Standardized across the board"@en;
	rdfs:label "Standardized"@en .

scm:state_salary
	a scm:IncomeSource ;
	rdfs:comment "can be paid either in currency or in kind (e.g., koku of rice)."@en ;
	rdfs:label "State Salary"@en .

scm:unitary_state
	a scm:DegreeOfCentralization ;
	rdfs:comment "regional governors are appointed and removed by the central authorities, taxes are imposed by, and transmitted to the center"@en ;
	rdfs:label "Unitary State"@en .

scm:unknown
   a scm:EpistemicState;
   rdfs:comment "It can be said with a high degree of confidence that it is not known whether the feature was present or absent in the context."@en ;
   rdfs:label "Unknown"@en .

scm:unstandardized
	a scm:Standardization ;
	rdfs:comment "Not standardized at all."@en;
	rdfs:label "Unstandardized"@en .

scm:vassalage
	a scm:SupraPolityRelations ;
	rdfs:comment "A central government exercises a certain degree of control, especially over military matters and international relations. Otherwise the polity is left alone"@en ;
	rdfs:label "Vassalage"@en .

scm:inferred
  rdfs:label "Inferred"@en ;
  rdfs:comment "The value has been logically inferred from other evidence"@en ;
  a scm:Confidence .

scm:disputed
  rdfs:label "Disputed"@en ;
  rdfs:comment "The evidence is disputed - some believe this data to be incorrect"@en ;
  a scm:Confidence .

scm:dubious
  rdfs:label "Dubious"@en ;
  rdfs:comment "The evidence is dubious - most believe this data to be incorrect"@en ;
  a scm:Confidence .

scm:uncertain
  rdfs:label "Uncertain"@en ;
  rdfs:comment "The evidence has a high degree of uncertainty"@en ;
  a scm:Confidence .

scm:unknown_identification
  rdfs:label "Unknown"@en ;
  rdfs:comment "How the leader is identified is unknown"@en ;
  a scm:LeaderIdentification .

scm:no_leader
  rdfs:label "No leader"@en ;
  rdfs:comment "There is no leader"@en ;
  a scm:LeaderIdentification .


scm:egalitarian_leadership
  rdfs:label "Egalitarian"@en ;
  rdfs:comment "Egalitarian leadership"@en ;
  a scm:LeaderIdentification .

scm:unknown_emphasis
  rdfs:label "Unknown"@en ;
  rdfs:comment "Unknown Emphasis"@en ;
  a scm:AuthorityEmphasis.


scm:unknown_epistemic_frequency
  rdfs:label "Unknown"@en ;
  rdfs:comment "Unknown Epistemic Frequency"@en ;
  a scm:EpistemicFrequency.


scm:unknown_frequency
  rdfs:label "Unknown"@en ;
  rdfs:comment "Unknown Frequency"@en ;
  a scm:Frequency.

scm:unknown_evolution
  rdfs:label "Unknown"@en ;
  rdfs:comment "Unknown Evolution"@en ;
  a scm:PoliticalEvolution.

scm:unknown_supra_polity_relations
  rdfs:label "Unknown"@en ;
  rdfs:comment "Unknown Relations"@en ;
  a scm:SupraPolityRelations.

scm:unknown_change
  rdfs:label "Unknown"@en ;
  rdfs:comment "Unknown Change"@en ;
  a scm:Change.

scm:never
  rdfs:label "Never"@en ;
  rdfs:comment "Never occurs"@en ;
  a scm:EpistemicFrequency.

scm:unknown_centralization
  rdfs:label "Unknown"@en ;
  rdfs:comment "Unknown Centralization"@en ;
  a scm:DegreeOfCentralization.

scm:unknown_complexity_change
  rdfs:label "Unknown"@en ;
  rdfs:comment "Unknown Change"@en ;
  a scm:ComplexityChange.

scm:unknown_income
  rdfs:label "Unknown"@en ;
  rdfs:comment "Unknown source of income"@en ;
  a scm:IncomeSource.

scm:unknown_sharing
  rdfs:label "Unknown"@en ;
  rdfs:comment "Unknown authority sharing"@en ;
  a scm:AuthoritySharing.

scm:egalitarian_sharing
  rdfs:label "Egalitarian"@en ;
  rdfs:comment "Egalitarian authority sharing"@en ;
  a scm:AuthoritySharing.

scm:egalitarian_contact
  rdfs:label "Egalitarian"@en ;
  rdfs:comment "Egalitarian contact access"@en ;
  a scm:ExternalContact.

scm:unknown_contact
  rdfs:label "Unknown"@en ;
  rdfs:comment "Unknown external contacts"@en ;
  a scm:ExternalContact.
	
scm:egalitarian_differentiation
  rdfs:label "Egalitarian"@en ;
  rdfs:comment "Egalitarian differentiation of leaders"@en ;
  a scm:LeaderDifferentiation.
	
scm:unknown_standardization
  rdfs:label "Unknown"@en ;
  rdfs:comment "Unknown standardization levels"@en ;
  a scm:Standardization.

scm:unknown_differentiation
  rdfs:label "Unknown"@en ;
  rdfs:comment "Unknown differentiation"@en ;
  a scm:Standardization.
